ModTuple2 compiles

compose/ModTuple2.v
@@ -13,6 +13,7 @@ Require Import AxiomsC.
 
 Require Import Mod Sem ModSem.
 Require Import Any.
+Require Import Program.
 
 Set Implicit Arguments.
 
@@ -84,6 +85,8 @@ Set Implicit Arguments.
 
 
 
+Global Unset Transparent Obligations.
+Add Search Blacklist "_obligation_".
 
 Lemma nth_error_nth
       X
@@ -101,32 +104,66 @@ Local Obligation Tactic := idtac.
 
 Variable ms_bot: ModSem.t.
 
-Module ModSem2.
+Section MODTUPLE.
 
-  Variable ms0 ms1: ModSem.t.
+  Variable skenv_link: SkEnv.t.
 
-  Definition owned_heap: Type := (ms0.(ModSem.owned_heap) * ms1.(ModSem.owned_heap)).
+  Variable link_skenv: SkEnv.t -> SkEnv.t -> SkEnv.t.
+
+  Variable msdl msdr: ModSem.t.
+
+  Hypothesis MIDXL: msdl.(ModSem.midx) <> None.
+  Hypothesis MIDXR: msdr.(ModSem.midx) <> None.
+
+  Definition owned_heap: Type := (msdl.(ModSem.owned_heap) * msdr.(ModSem.owned_heap)).
   
   Definition initial_owned_heap: owned_heap :=
-    (ms0.(ModSem.initial_owned_heap), ms1.(ModSem.initial_owned_heap)).
+    (msdl.(ModSem.initial_owned_heap), msdr.(ModSem.initial_owned_heap)).
 
-  Definition genvtype: Type := (ms0.(ModSem.genvtype) * ms1.(ModSem.genvtype)).
+  Definition genvtype: Type := (msdl.(ModSem.genvtype) * msdr.(ModSem.genvtype)).
 
-  Set Printing Universes.
+  Definition globalenv: genvtype := (msdl.(ModSem.globalenv), msdr.(ModSem.globalenv)).
+
+  (* Set Printing Universes. *)
+
+  Variant dir: Type :=
+  | dl
+  | dr
+  .
 
   Inductive stack: Type :=
   | StackNil
-      (oh: owned_heap)
   | StackCons
-      (b: bool)
-      (st0: (if b then ms0 else ms1).(ModSem.state))
+      (d: dir)
+      (st0: (if d then msdl else msdr).(ModSem.state))
+      (* (st0: msdl.(ModSem.state) + msdr.(ModSem.state)) *)
       (tl: stack)
   .
 
+  Lemma stack_inj
+        b0 hd0 tl0 b1 hd1 tl1
+        (EQ: (StackCons b0 hd0 tl0) = (StackCons b1 hd1 tl1))
+    :
+      b0 = b1 /\ hd0 ~= hd1 /\ tl0 = tl1
+  .
+  Proof.
+    des_ifs; simpl_depind; clarify; esplits; eauto.
+  Qed.
+
+  Lemma state_inj
+        b0 hd0 tl0 (ohs0: owned_heap) b1 hd1 tl1 ohs1
+        (EQ: ((StackCons b0 hd0 tl0), ohs0) = ((StackCons b1 hd1 tl1), ohs1))
+    :
+      b0 = b1 /\ hd0 ~= hd1 /\ tl0 = tl1 /\ ohs0 = ohs1
+  .
+  Proof.
+    des_ifs; simpl_depind; clarify; esplits; eauto.
+  Qed.
+
   Definition state: Type := (stack * owned_heap).
 
-  (* Definition ms (b: bool): ModSem.t := (if b then ms0 else ms1). *)
-  Notation ms := (fun (b: bool) => (if b then ms0 else ms1)).
+  (* Definition ms (b: bool): ModSem.t := (if b then msdl else msdr). *)
+  Notation ms := (fun (b: bool) => (if b then msdl else msdr)).
 
   Definition update A B (b: bool) (x: if b then A else B) (ab: A * B): A * B :=
     (if b as b0 return ((if b0 then A else B) -> A * B)
@@ -139,113 +176,224 @@ Don't want to split call/init step, because we have to define Callstate separate
 To do this, I will require initial_state to be deterministic.
    ***)
 
-  Inductive step (se: Senv.t) (ge: genvtype): state -> trace -> state -> Prop :=
-  | step_call
-      (b: bool) st0 st1 tl oh ohs0 ohs1 args
-      (AT: (ms b).(ModSem.at_external) st0 oh args)
-      (OHS: update b oh ohs0 = ohs1)
-    :
-    step se ge ((StackCons b st0 tl), ohs0)
-         E0 ((StackCons b st1 (StackCons b st0 tl)), ohs1)
-  | step_internal
-      (b: bool) st0 tr st1 tl ohs
-      (STEP: ModSem.step (ms b) ((ms b).(ModSem.skenv_link)) ((ms b).(ModSem.globalenv)) st0 tr st1)
-    :
-      step se ge ((StackCons b st0 tl), ohs)
-           tr ((StackCons b st1 tl), ohs)
-  .
-
-
-
-
-
-  Inductive state: Type :=
-  | StateNil
-  | StateCons
-      (* (b: bool) *)
-      (* (st0: (if b then ms0 else ms1).(ModSem.state)) *)
-      (st0: ms0.(ModSem.state) + ms1.(ModSem.state))
-      (tl: state)
-  .
-
-  Inductive find_fptr_owner (fptr: val) (ms: ModSem.t): Prop :=
+  Variant find_fptr_owner (fptr: val) (ms: ModSem.t): Prop :=
   | find_fptr_owner_intro
-      (MODSEM: In ms [ms0 ; ms1])
+      (MODSEM: In ms [msdl ; msdr])
       if_sig
       (INTERNAL: Genv.find_funct ms.(ModSem.skenv) fptr = Some (Internal if_sig)).
 
-  Inductive step (se: Senv.t) (ge: genvtype): state -> trace -> state -> Prop :=
-  (* | step_internal *)
-  (*     (b: bool) (st0 st1: ModSem.state (if b then ms0 else ms1)) tr tl *)
-  (*     (STEP: Smallstep.step (if b then ms0 else ms1) st0 tr st1) *)
-  (*   : *)
-  (*     step se ge (StateCons b st0 tl) *)
-  (*          tr (StateCons b st1 tl) *)
+  Variant step (se: Senv.t) (ge: genvtype): state -> trace -> state -> Prop :=
+  | step_call_dl
+      st0 st_new tl oh0 oh_new ohs0 ohs1 args
+      (AT: msdl.(ModSem.at_external) st0 oh0 args)
+      (OHS: ohs1 = (oh0, snd ohs0))
 
-
-  (* | step_internal *)
-  (*     (b: bool) (st0 st1: (if b then ms0.(ModSem.state) else ms1.(ModSem.state))) tr tl *)
-  (*     (STEP: if b then Step ms0 st0 tr st1 else Step ms1 st0 tr st1) *)
-  (*   : *)
-  (*     step se ge (StateCons b st0 tl) *)
-  (*          tr (StateCons b st1 tl) *)
-
-
-  | step_internal_l
-      st0 tr st1 tl
-      (STEP: Step ms0 st0 tr st1)
+      (MSFIND: find_fptr_owner (Args.get_fptr args) msdr)
+      (OH: snd ohs1 = oh_new)
+      (INIT: msdr.(ModSem.initial_frame) oh_new args st_new)
     :
-      step se ge (StateCons (inl st0) tl)
-           tr (StateCons (inl st1) tl)
-  | step_internal_r
-      st0 tr st1 tl
-      (STEP: Step ms1 st0 tr st1)
+    step se ge ((StackCons dl st0 tl), ohs0)
+         E0 ((StackCons dr st_new (StackCons dl st0 tl)), ohs1)
+
+  | step_internal_dl
+      st0 tr st1 tl ohs
+      (STEP: Step msdl st0 tr st1)
     :
-      step se ge (StateCons (inr st0) tl)
-           tr (StateCons (inr st1) tl)
+      step se ge ((StackCons dl st0 tl), ohs)
+           tr ((StackCons dl st1 tl), ohs)
+
+  | step_return_dl
+      st_old st0 st1 tl oh0 oh_old ohs0 ohs1 retv
+      (AT: msdl.(ModSem.final_frame) st0 oh0 retv)
+      (OHS: ohs1 = (oh0, snd ohs0))
+
+      (OH: snd ohs1 = oh_old)
+      (INIT: msdr.(ModSem.after_external) st_old oh_old retv st1)
+    :
+    step se ge ((StackCons dl st0 (StackCons dr st_old tl)), ohs0)
+         E0 ((StackCons dr st1 tl), ohs1)
+
+
+  (* | step_internal *)
+  (*     (b: bool) st0 tr st1 tl ohs *)
+  (*     (STEP: ModSem.step (ms b) ((ms b).(ModSem.skenv_link)) ((ms b).(ModSem.globalenv)) st0 tr st1) *)
+  (*   : *)
+  (*     step se ge ((StackCons b st0 tl), ohs) *)
+  (*          tr ((StackCons b st1 tl), ohs) *)
+
+  | step_call_dr
+      st0 st_new tl oh0 oh_new ohs0 ohs1 args
+      (AT: msdr.(ModSem.at_external) st0 oh0 args)
+      (OHS: ohs1 = (fst ohs0, oh0))
+
+      (MSFIND: find_fptr_owner (Args.get_fptr args) msdr)
+      (OH: fst ohs1 = oh_new)
+      (INIT: msdl.(ModSem.initial_frame) oh_new args st_new)
+    :
+    step se ge ((StackCons dr st0 tl), ohs0)
+         E0 ((StackCons dl st_new (StackCons dr st0 tl)), ohs1)
+
+  | step_internal_dr
+      st0 tr st1 tl ohs
+      (STEP: Step msdr st0 tr st1)
+    :
+      step se ge ((StackCons dr st0 tl), ohs)
+           tr ((StackCons dr st1 tl), ohs)
+
+  | step_return_dr
+      st_old st0 st1 tl oh0 oh_old ohs0 ohs1 retv
+      (AT: msdr.(ModSem.final_frame) st0 oh0 retv)
+      (OHS: ohs1 = (fst ohs0, oh0))
+
+      (OH: fst ohs1 = oh_old)
+      (INIT: msdl.(ModSem.after_external) st_old oh_old retv st1)
+    :
+    step se ge ((StackCons dr st0 (StackCons dl st_old tl)), ohs0)
+         E0 ((StackCons dl st1 tl), ohs1)
   .
 
-  (* Inductive step' (se: Senv.t) (ge: genvtype) (st0: state) (tr: trace) (st1: state): Prop := *)
-  (* | step'_internal *)
-  (*     n *)
-  (*     (NTH: match (nth_error mss n) with *)
-  (*           | Some ms => *)
-  (*             exists (hd0 hd1: ms.(ModSem.state)), *)
-  (*               <<STK0: hd_error (get_stk st0) = Some (upcast (n, hd0))>> /\ *)
-  (*               (* <<STK0: hd_error (get_stk st0) = Some (upcast (n, hd0))>> /\ *) *)
-  (*               (* <<STK1: hd_error (get_stk st1) = Some (upcast (n, hd1))>> /\ *) *)
-  (*               <<OH: get_ohs st0 = get_ohs st1>> /\ *)
-  (*               <<STEP: Step ms hd0 tr hd1>> *)
-  (*           | _ => False *)
-  (*           end *)
-  (*     ) *)
-  (* . *)
-  (* Reset step'. *)
+  Variant at_external: state -> owned_heap -> Args.t -> Prop :=
+  | at_external_dl
+      st0 tl oh0 ohs0 args
+      (AT: msdl.(ModSem.at_external) st0 oh0 args)
+      (MSFIND: forall msdr, ~find_fptr_owner (Args.get_fptr args) msdr)
+    :
+      at_external ((StackCons dl st0 tl), ohs0) (oh0, snd ohs0) args
 
-  (* Print Universes. *)
+  | at_external_dr
+      st0 tl oh0 ohs0 args
+      (AT: msdr.(ModSem.at_external) st0 oh0 args)
+      (MSFIND: forall msdl, ~find_fptr_owner (Args.get_fptr args) msdl)
+    :
+      at_external ((StackCons dr st0 tl), ohs0) (fst ohs0, oh0) args
+  .
 
-  Variable skenv_link: SkEnv.t.
+  Variant initial_frame (ohs: owned_heap) (args: Args.t): state -> Prop :=
+  | initial_frame_dl
+      st0
+      (MSFIND: find_fptr_owner (Args.get_fptr args) msdl)
+      (INIT: msdl.(ModSem.initial_frame) (fst ohs) args st0)
+    :
+      initial_frame ohs args (StackCons dl st0 StackNil, ohs)
 
-  Variable link_skenv: SkEnv.t -> SkEnv.t -> SkEnv.t.
+  | initial_frame_dr
+      st0
+      (MSFIND: find_fptr_owner (Args.get_fptr args) msdr)
+      (INIT: msdr.(ModSem.initial_frame) (snd ohs) args st0)
+    :
+      initial_frame ohs args (StackCons dr st0 StackNil, ohs)
+  .
 
-  Set Printing Universes.
-  Print Universes.
+  Variant final_frame: state -> owned_heap -> Retv.t -> Prop :=
+  | final_frame_dl
+      st0 retv ohs0 oh0
+      (FINAL: msdl.(ModSem.final_frame) st0 oh0 retv)
+    :
+      final_frame (StackCons dl st0 StackNil, ohs0) (oh0, snd ohs0) retv
 
-  Program Definition t': ModSem.t :=
+  | final_frame_dr
+      st0 retv ohs0 oh0
+      (FINAL: msdr.(ModSem.final_frame) st0 oh0 retv)
+    :
+      final_frame (StackCons dr st0 StackNil, ohs0) (fst ohs0, oh0) retv
+  .
+
+  Variant after_external: state -> owned_heap -> Retv.t -> state -> Prop :=
+  | after_external_dl
+      tl st0 ohs0 ohs1 retv st1
+      (AFTER: msdl.(ModSem.after_external) st0 (fst ohs1) retv st1)
+    :
+      after_external (StackCons dl st0 tl, ohs0) ohs1 retv (StackCons dl st1 tl, ohs1)
+
+  | after_external_dr
+      tl st0 ohs0 ohs1 retv st1
+      (AFTER: msdr.(ModSem.after_external) st0 (snd ohs1) retv st1)
+    :
+      after_external (StackCons dr st0 tl, ohs0) ohs1 retv (StackCons dr st1 tl, ohs1)
+  .
+
+  Program Definition t: ModSem.t :=
     {|
       ModSem.state := state;
       ModSem.owned_heap := owned_heap;
       ModSem.genvtype := genvtype;
-      (* ModSem.step := step; *)
-      (* ModSem.at_external := coerce at_external; *)
-      (* ModSem.initial_frame := coerce initial_frame; *)
-      (* ModSem.final_frame := coerce final_frame; *)
-      (* ModSem.after_external := ms0.(ModSem.after_external); *)
-      (* ModSem.globalenv := ge; *)
-      (* ModSem.skenv := link_skenv ms0.(ModSem.skenv) ms1.(ModSem.skenv); *)
-      (* ModSem.skenv_link := skenv_link; *)
-      (* ModSem.midx := None; *)
+      ModSem.step := step;
+      ModSem.at_external := at_external;
+      ModSem.initial_frame := initial_frame;
+      ModSem.final_frame := final_frame;
+      ModSem.after_external := after_external;
+      ModSem.initial_owned_heap := initial_owned_heap;
+      ModSem.globalenv := globalenv;
+      ModSem.skenv := link_skenv msdl.(ModSem.skenv) msdr.(ModSem.skenv);
+      ModSem.skenv_link := skenv_link;
+      ModSem.midx := msdl.(ModSem.midx); (*** <-- TODO: prettify later ***)
     |}
   .
+  Next Obligation.
+    ii.
+    inv AT0.
+    - remember (StackCons dl st0 tl, ohs0) as Y.
+      inv AT1; ss. eapply state_inj in H. des; clarify.
+      determ_tac ModSem.at_external_dtm; esplits; et.
+    - remember (StackCons dr st0 tl, ohs0) as Y.
+      inv AT1; ss. eapply state_inj in H. des; clarify.
+      determ_tac ModSem.at_external_dtm; esplits; et.
+  Qed.
+  Next Obligation.
+    ii.
+    inv FINAL0.
+    - remember (StackCons dl st0 StackNil, ohs0) as Y.
+      inv FINAL1; ss. eapply state_inj in H. des; clarify.
+      determ_tac ModSem.final_frame_dtm; esplits; et.
+    - remember (StackCons dr st0 StackNil, ohs0) as Y.
+      inv FINAL1; ss. eapply state_inj in H. des; clarify.
+      determ_tac ModSem.final_frame_dtm; esplits; et.
+  Qed.
+  Next Obligation.
+    ii.
+    inv AFTER0.
+    - remember (StackCons dl st2 tl, ohs0) as Y.
+      inv AFTER1; ss. eapply state_inj in H. des; clarify.
+      determ_tac ModSem.after_external_dtm; esplits; et.
+    - remember (StackCons dr st2 tl, ohs0) as Y.
+      inv AFTER1; ss. eapply state_inj in H. des; clarify.
+      determ_tac ModSem.after_external_dtm; esplits; et.
+  Qed.
+  Next Obligation.
+    ii. rr. des.
+    pose x0 as X.
+    inv PR.
+    - remember (StackCons dl st0 tl, ohs0) as Y.
+      inv PR0; ss; eapply state_inj in H; des; clarify; try (by ModSem.tac).
+      determ_tac ModSem.at_external_dtm. eapply MSFIND; eauto.
+    - remember (StackCons dr st0 tl, ohs0) as Y.
+      inv PR0; ss; eapply state_inj in H; des; clarify; try (by ModSem.tac).
+      determ_tac ModSem.at_external_dtm. eapply MSFIND; eauto.
+  Qed.
+  Next Obligation.
+    ii. rr. des.
+    pose x0 as X.
+    inv PR0.
+    - remember (StackCons dl st0 StackNil, ohs0) as Y.
+      inv PR; ss; eapply state_inj in H; des; clarify; try (by ModSem.tac).
+    - remember (StackCons dr st0 StackNil, ohs0) as Y.
+      inv PR; ss; eapply state_inj in H; des; clarify; try (by ModSem.tac).
+  Qed.
+  Next Obligation.
+    ii. rr. des.
+    pose x0 as X.
+    inv PR.
+    - remember (StackCons dl st0 tl, ohs0) as Y.
+      inv PR0; ss; eapply state_inj in H; des; clarify; try (by ModSem.tac).
+    - remember (StackCons dr st0 tl, ohs0) as Y.
+      inv PR0; ss; eapply state_inj in H; des; clarify; try (by ModSem.tac).
+  Qed.
+  Next Obligation.
+    i. ss.
+  Qed.
 
-End ModSem2.
+End MODTUPLE.
+
+Module ModTuple.
+  Definition t := Eval red in t.
+End ModTuple.
